Remove local_funspec.

veric/semax_ext.v
@@ -21,25 +21,27 @@ Variable Z : Type.
 
 Variable Espec : juicy_ext_spec Z.
 
-Definition funspec2types id (A : Type) (ef : external_function) : Type :=
-  if ident_eq id (ef_id ef) then A else (ext_spec_type Espec ef).
-
 Parameter symb2genv : forall (ge_s : PTree.t block), genv. (*TODO*)
 Axiom symb2genv_ax : forall (ge_s : PTree.t block), Genv.genv_symb (symb2genv ge_s) = ge_s.
 
 Definition funspec2pre (A : Type) P id ef x ge_s (tys : list typ) args (z : Z) m : Prop :=
   match ident_eq id (ef_id ef) as s 
-  return ((if s then A else ext_spec_type Espec ef) -> Prop)
+  return ((if s then (rmap*A)%type else ext_spec_type Espec ef) -> Prop)
   with 
-    | left _ => fun x' => P x' (make_ext_args (symb2genv ge_s) 1 args) (m_phi m)
+    | left _ => fun x' => exists phi0 phi1, join phi0 phi1 (m_phi m) 
+                       /\ P (snd x') (make_ext_args (symb2genv ge_s) 1 args) phi0
+                       /\ necR (fst x') phi1 
     | right n => fun x' => ext_spec_pre Espec ef x' ge_s tys args z m
   end x.
 
-Definition funspec2post (A : Type) Q id ef x (tret : option typ) ret (z : Z) m : Prop :=
+Definition funspec2post (A : Type) (Q : A -> environ -> mpred) 
+                        id ef x (tret : option typ) ret (z : Z) m : Prop :=
   match ident_eq id (ef_id ef) as s 
-  return ((if s then A else ext_spec_type Espec ef) -> Prop)
+  return ((if s then (rmap*A)%type else ext_spec_type Espec ef) -> Prop)
   with 
-    | left _ => fun x' => Q x' (make_ext_rval 1 ret) (m_phi m)
+    | left _ => fun x' => exists phi0 phi1, join phi0 phi1 (m_phi m) 
+                       /\ Q (snd x') (make_ext_rval 1 ret) phi0
+                       /\ necR (fst x') phi1 
     | right n => fun x' => ext_spec_post Espec ef x' tret ret z m
   end x.
 
@@ -48,7 +50,7 @@ Definition funspec2extspec (f : (ident*funspec))
   match f with 
     | (id, mk_funspec sig A P Q) =>
       Build_external_specification juicy_mem external_function Z
-        (fun ef => if ident_eq id (ef_id ef) then A else ext_spec_type Espec ef)
+        (fun ef => if ident_eq id (ef_id ef) then (rmap*A)%type else ext_spec_type Espec ef)
         (funspec2pre A P id)
         (funspec2post A Q id)
         (fun rv z m => False)
@@ -77,7 +79,14 @@ destruct f; simpl; unfold funspec2pre; simpl.
 simpl in t; revert t.
 destruct (ident_eq i (ef_id e)).
 * clear wf; subst i; intros t a a' Hage; destruct m; simpl.
-solve[apply h; apply age_jm_phi; auto].
+intros [phi0 [phi1 [Hjoin [Hx Hy]]]].
+apply age1_juicy_mem_unpack in Hage.
+destruct Hage as [Hage Hdry].
+destruct (age1_join2 phi0 Hjoin Hage) as [x' [y' [Hjoin' [Hage' H]]]].
+exists x', y'; split; auto.
+split; [solve[eapply h; eauto]|].
+apply (necR_trans (fst t) phi1 y'); auto.
+unfold necR. constructor; auto.
 * intros ? ? ?; auto.
 destruct Espec; simpl; apply JE_pre_hered.
 Qed.
@@ -86,7 +95,14 @@ destruct f; simpl; unfold funspec2post; simpl.
 simpl in t; revert t.
 destruct (ident_eq i (ef_id e)).
 * clear wf; subst i; intros t a a' Hage; destruct m0; simpl.
-apply h; apply age_jm_phi; auto.
+intros [phi0 [phi1 [Hjoin [Hx Hy]]]].
+apply age1_juicy_mem_unpack in Hage.
+destruct Hage as [Hage Hdry].
+destruct (age1_join2 phi0 Hjoin Hage) as [x' [y' [Hjoin' [Hage' H]]]].
+exists x', y'; split; auto.
+split; [solve[eapply h; eauto]|].
+apply (necR_trans (fst t) phi1 y'); auto.
+unfold necR. constructor; auto.
 * intros ? ? ?; auto.
 destruct Espec; simpl; apply JE_post_hered.
 Qed.
@@ -100,8 +116,21 @@ unfold funspec2pre, funspec2post.
 destruct (ident_eq i (ef_id e)).
 * intros. intros adr.
 destruct H2 as [H2 _].
-specialize (H2 t (make_ext_args (symb2genv ge_s) 1 args) (make_ext_rval 1 rv)). 
-apply (H2 (m_phi jm) (m_phi jm') H H0 adr).
+specialize (H2 (snd t) (make_ext_args (symb2genv ge_s) 1 args) (make_ext_rval 1 rv)). 
+destruct H as [phi0 [phi1 [Hjoin [Hpre Hnec]]]].
+destruct H0 as [phi0' [phi1' [Hjoin' [Hpost Hnec']]]].
+generalize (H2 _ _ Hpre Hpost adr). clear H2.
+clear -Hjoin Hjoin'. 
+cut (level phi0' = level jm'). intros Hlev.
+apply resource_at_join with (loc := adr) in Hjoin. revert Hjoin.
+apply resource_at_join with (loc := adr) in Hjoin'. revert Hjoin'.
+case_eq (m_phi jm @ adr); auto. intros k p Hpure.
+case_eq (phi0 @ adr); try solve[inversion 3].
+intros ? ? Hphi0. inversion 2. subst.
+intros H2; rewrite H2 in Hjoin'. inv Hjoin'. rewrite Hlev.
+rewrite level_juice_level_phi; auto.
+apply join_level in Hjoin'. 
+destruct Hjoin'; auto.
 * destruct Espec; simpl; intros.
 clear H2; eapply (JE_rel e); eauto.
 Qed.
@@ -159,30 +188,32 @@ Fixpoint add_funspecs_rec (Z : Type) (Espec : juicy_ext_spec Z) (fs : wf_funspec
 
 Require Import JMeq.
 
-Lemma add_funspecs_pre {Z fs id sig A P Q x args m} Espec tys ge_s :
+Lemma add_funspecs_pre {Z fs id sig A P Q x args m} Espec tys ge_s phi0 phi1 :
   let ef := EF_external id (funsig2signature sig) in
   funspecs_norepeat fs -> 
   in_funspecs (id, (mk_funspec sig A P Q)) fs -> 
-  P x (make_ext_args (symb2genv ge_s) 1%positive args) (m_phi m) ->
+  join phi0 phi1 (m_phi m) ->
+  P x (make_ext_args (symb2genv ge_s) 1%positive args) phi0 ->
   exists x' : ext_spec_type (JE_spec _ (add_funspecs_rec Z Espec fs)) ef, 
-    JMeq x x' /\ forall z, ext_spec_pre (add_funspecs_rec Z Espec fs) ef x' ge_s tys args z m.
+    JMeq (phi1,x) x' 
+    /\ forall z, ext_spec_pre (add_funspecs_rec Z Espec fs) ef x' ge_s tys args z m.
 Proof.
-induction fs; [intros; elimtype False; auto|]; intros ef H H1 H2.
+induction fs; [intros; elimtype False; auto|]; intros ef H H1 H2 Hpre.
 destruct H1 as [H1|H1].
 
 { 
 subst f;simpl in *.
-clear IHfs H; revert x H2; unfold funspec2pre; simpl.
+clear IHfs H; revert x H2 Hpre; unfold funspec2pre; simpl.
 destruct (ident_eq id id); simpl.
-solve[intros x Hp; exists x; auto].
-solve[elimtype False; auto]. 
+intros x Hjoin Hp. exists (phi1,x). split; eauto.
+elimtype False; auto.
 }
 
 { 
 assert (Hin: in_funspecs_by_id (id, mk_funspec sig A P Q) fs). 
 { clear -H1; apply in_funspecs_in_by_id in H1; auto. }
 destruct H as [Ha Hb]. 
-destruct (IHfs Hb H1 H2) as [x' H3].
+destruct (IHfs Hb H1 H2 Hpre) as [x' H3].
 clear -Ha Hin H1 H3; revert x' Ha Hin H1 H3.
 destruct f; simpl; destruct f; simpl; unfold funspec2pre; simpl.
 destruct (ident_eq i id).
@@ -199,25 +230,30 @@ Lemma add_funspecs_post {Z Espec tret fs id sig A P Q x ret m z} :
   funspecs_norepeat fs -> 
   in_funspecs (id, (mk_funspec sig A P Q)) fs -> 
   ext_spec_post (add_funspecs_rec Z Espec fs) ef x tret ret z m -> 
-  exists x' : A, 
-    JMeq x x' /\ Q x' (make_ext_rval 1%positive ret) (m_phi m).
+  exists (phi0 phi1 phi1' : rmap) (x' : A), 
+       join phi0 phi1 (m_phi m) 
+    /\ necR phi1' phi1
+    /\ JMeq x (phi1',x') 
+    /\ Q x' (make_ext_rval 1%positive ret) phi0.
 Proof.
-induction fs; [intros; elimtype False; auto|]; intros ef H H1 H2.
+induction fs; [intros; elimtype False; auto|]; intros ef H H1 Hpost.
 destruct H1 as [H1|H1].
 
 { 
 subst f;simpl in *.
-clear IHfs H; revert x H2; unfold funspec2post; simpl.
+clear IHfs H; revert x Hpost; unfold funspec2post; simpl.
 destruct (ident_eq id id); simpl.
-solve[intros x Hp; exists x; auto].
-solve[elimtype False; auto]. 
+intros x [phi0 [phi1 [Hjoin [Hq Hnec]]]].
+exists phi0, phi1, (fst x), (snd x).
+split; auto. split; auto. destruct x; simpl in *. split; auto.
+elimtype False; auto.
 }
 
 { 
 assert (Hin: in_funspecs_by_id (id, mk_funspec sig A P Q) fs). 
 { clear -H1; apply in_funspecs_in_by_id in H1; auto. }
 destruct H as [Ha Hb]. 
-clear -Ha Hin H1 H2 Hb IHfs; revert x Ha Hin H1 H2 Hb IHfs.
+clear -Ha Hin H1 Hb Hpost IHfs; revert x Ha Hin H1 Hb Hpost IHfs.
 destruct f; simpl; destruct f; simpl; unfold funspec2post; simpl.
 destruct (ident_eq i id).
 * subst i; destruct fs; [solve[simpl; intros; elimtype False; auto]|].
@@ -234,42 +270,26 @@ Definition add_funspecs (Espec : OracleKind) (fs : wf_funspecs) : OracleKind :=
       Build_OracleKind ty (add_funspecs_rec ty spec fs)
   end.
 
-Definition local_funspec (f : funspec) :=
-  match f with mk_funspec spec A P Q => 
-      (* safety monotonicity *)
-      (forall (x : A) rho phi1 phi2 phi, join phi1 phi2 phi -> 
-         P x rho phi1 -> P x rho phi)
-      (* frame property *)
-   /\ (forall (x : A) rho phi1 phi2 phi, join phi1 phi2 phi -> 
-         P x rho phi1 -> 
-       forall rho' phi', (level phi >= level phi')%nat -> 
-         Q x rho' phi' ->
-         exists phi1' phi2', 
-         join phi1' phi2' phi' /\ age phi2 phi2' /\ Q x rho' phi1')         
-  end.
-
 Section semax_ext.
 
 Variable Espec : OracleKind.
 
 Lemma semax_ext id sig A P Q (fs : wf_funspecs) : 
   let f := mk_funspec sig A P Q in
-  local_funspec f -> 
   in_funspecs (id,f) fs -> 
   funspecs_norepeat fs -> 
   (forall n, semax_external (add_funspecs Espec fs) (EF_external id (funsig2signature sig)) _ P Q n).
 Proof.
-intros f Hloc Hin Hnorepeat.
+intros f Hin Hnorepeat.
 unfold semax_external.
 intros n ge x n0 Hlater F ts args jm H jm' H2 H3.
 destruct H3 as [s [t [Hjoin [Hp Hf]]]].
-cut (P x (make_ext_args ge 1 args) (m_phi jm')). intro Hp'.
 destruct Espec.
-assert (Hp'': P x (make_ext_args (symb2genv (Genv.genv_symb ge)) 1 args) (m_phi jm')).
+assert (Hp'': P x (make_ext_args (symb2genv (Genv.genv_symb ge)) 1 args) s).
 { generalize (in_funspecs_wf _ _ Hin). simpl; intros [Hwf1 Hwf2].
   rewrite Hwf2; eauto.
   rewrite symb2genv_ax; auto. }
-destruct (add_funspecs_pre OK_spec ts (Genv.genv_symb ge) Hnorepeat Hin Hp'') 
+destruct (add_funspecs_pre OK_spec ts (Genv.genv_symb ge) s t Hnorepeat Hin Hjoin Hp'') 
   as [x' [Heq Hpre]].
 simpl.
 exists x'.
@@ -277,24 +297,14 @@ intros z.
 split; [solve[apply Hpre]|].
 intros tret ret z' jm2 Hlev jm3 Hnec Hpost.
 
-cut (Q x (make_ext_rval 1 ret) (m_phi jm3)). intro Hq.
-unfold f in Hloc.
-destruct Hloc as [Hl1 Hl2].
-assert (Hlev': (level (m_phi jm') >= level (m_phi jm3))%nat). 
-{ cut ((level (m_phi jm2) >= level (m_phi jm3))%nat). omega.
-  apply necR_level in Hnec; erewrite <-level_juice_level_phi; eauto. }
-destruct (Hl2 _ _ s t (m_phi jm') Hjoin Hp _ _ Hlev' Hq) 
-  as [phi' [t' [Hjoin' [Hage' Hq']]]].
-exists phi', t'; split; auto.
-split; auto. destruct F. simpl in Hf|-*. eapply h in Hf; eauto.
-
 eapply add_funspecs_post in Hpost; eauto.
-destruct Hpost as [x'' [Heq' Hq']].
-assert (JMeq x x'') by (eapply JMeq_trans; eauto).
-solve[apply JMeq_eq in H0; subst; auto].
-
-unfold f in Hloc; destruct Hloc as [Hloc _]. 
-solve[eapply Hloc; eauto].
+destruct Hpost as [phi0 [phi1 [phi1' [x'' [Hjoin' [Hnec' [Hjmeq' Hq']]]]]]].
+exists phi0, phi1; split; auto.
+assert (JMeq (t,x) (phi1',x'')) by (eapply JMeq_trans; eauto).
+assert ((t,x) = (phi1',x'')) by (apply JMeq_eq in H0; auto).
+inv H1.
+split; auto.
+eapply pred_nec_hereditary; eauto.
 Qed.
   
 End semax_ext.  
