veric/SeparationLogic.v
@@ -908,7 +908,6 @@ Require veric.semax_ext.
 Definition wf_funspec := veric.semax_ext.wf_funspec.
 Definition wf_funspecs := veric.semax_ext.wf_funspecs.
 Definition in_funspecs := veric.semax_ext.in_funspecs.
-Definition local_funspec := veric.semax_ext.local_funspec.
 Definition funspecs_norepeat := veric.semax_ext.funspecs_norepeat.
 Definition add_funspecs := veric.semax_ext.add_funspecs.
 Definition funsig2signature := veric.semax_ext.funsig2signature.
@@ -918,7 +917,6 @@ Axiom semax_ext:
          (id : ident) (sig : funsig) 
          (A : Type) (P Q : A -> environ -> mpred) (fs : wf_funspecs),
     let f := mk_funspec sig A P Q in
-    local_funspec f ->
     in_funspecs (id, f) fs ->
     funspecs_norepeat fs ->
     @semax_external (add_funspecs Espec fs) (EF_external id (funsig2signature sig)) A P Q.
